adapted up to the small step semantics

program.v
@@ -20,7 +20,6 @@ Require Import Coq.Structures.OrdersEx.      (* Provides New Keys *)
 Global Open Scope string_scope.
 Global Open Scope Z_scope.
 
- 
 (* A module for block identifier *)
 Module BlockID.
   (* A block ID is a natural number using N ofr effciency. *)
@@ -67,7 +66,7 @@ Module BlockID.
 End BlockID.
 
 
-Module YULVariable.
+Module VarID.
   (* YUL variables are represented as natural numbers using N for efficiency. *)
   Definition t := N.
 
@@ -110,20 +109,20 @@ Module YULVariable.
   Defined.
 
  (* It is a UsualOrderedType, we simply use that of N *)
-  Module YULVariable_as_OT := OrdersEx.N_as_OT.
-End YULVariable.
+  Module VarID_as_OT := OrdersEx.N_as_OT.
+End VarID.
 
 (* This module defines a set of variables. It is not used here, the
 purpose is to use it in analysis that requires such sets. *)
-Module YULVarSet := MSetAVL.Make(YULVariable.YULVariable_as_OT).
+Module VarIDSet := MSetAVL.Make(VarID.VarID_as_OT).
 
 (* This module defines simple expressions, which can be a variable or a value *)
 Module SimpleExpr (D: DIALECT).
-  Definition t : Type := YULVariable.t + D.value_t.
+  Definition t : Type := VarID.t + D.value_t.
 
   Definition eqb (x y: t): bool :=
     match x, y with
-    | inl v1, inl v2 => YULVariable.eqb v1 v2
+    | inl v1, inl v2 => VarID.eqb v1 v2
     | inr v1, inr v2 => D.eqb v1 v2
     | _,_ => false
     end.
@@ -134,17 +133,17 @@ Module SimpleExpr (D: DIALECT).
     intros x y.
     unfold eqb.
     destruct x as [xvar | xval]; destruct y as [yvar | yval].
-    - destruct (YULVariable.eqb_spec xvar yvar) as [Heq | Hneq].
-      + rewrite <- YULVariable.eqb_eq in Heq.
+    - destruct (VarID.eqb_spec xvar yvar) as [Heq | Hneq].
+      + rewrite <- VarID.eqb_eq in Heq.
         rewrite Heq.
         apply ReflectT.
-        rewrite YULVariable.eqb_eq in Heq.
+        rewrite VarID.eqb_eq in Heq.
         rewrite Heq.
         reflexivity.
-      + rewrite <- YULVariable.eqb_neq_false in Hneq.
+      + rewrite <- VarID.eqb_neq_false in Hneq.
         rewrite Hneq.
         apply ReflectF.
-        rewrite YULVariable.eqb_neq_false in Hneq.
+        rewrite VarID.eqb_neq_false in Hneq.
         intro H_contra.
         injection H_contra as H_contra.
         contradiction.
@@ -202,7 +201,7 @@ Module SimpleExpr (D: DIALECT).
 
 End SimpleExpr.
 
-Module FunctionName.
+Module FuncID.
   (* YUL Function names represented as strings. *)
   Definition t := string.
 
@@ -244,7 +243,7 @@ Module FunctionName.
     Misc.sumbool_from_reflect (eqb_spec x y).
   Defined.
 
-End FunctionName.
+End FuncID.
 
 
 
@@ -253,43 +252,45 @@ Module ExitInfo (D: DIALECT).
   Module SimpleExprD := SimpleExpr(D).
   
   Inductive t : Type := 
-  | ConditionalJump (cond_var : YULVariable.t) (target_if_true : BlockID.t) (target_if_false : BlockID.t)
-  | Jump (target : BlockID.t)
-  | ReturnBlock (return_values : list SimpleExprD.t)
-  | Terminated.
+  | ConditionalJump (cond_var_id : VarID.t) (bid_if_true : BlockID.t) (bid_if_false : BlockID.t)
+  | Jump (bid : BlockID.t)
+  | ReturnBlock (ret_eexprs : list SimpleExprD.t)
+  | Terminate.
 
 End ExitInfo.
 
-Search (NoDup nil).
 
 Module PhiInfo (D: DIALECT).
 
   Module SimpleExprD := SimpleExpr(D).
 
   Inductive InBlockPhiInfo :=
-  | in_phi_info (out_vars: list YULVariable.t) (in_vars: list SimpleExprD.t) (H_no_dup: List.NoDup out_vars) (H_same_le: length out_vars = length in_vars).
+  | in_phi_info (out_vars: list VarID.t) (in_sexprs: list SimpleExprD.t) (H_no_dup: List.NoDup out_vars) (H_same_le: length out_vars = length in_sexprs).
   
   Definition t := BlockID.t -> InBlockPhiInfo.
 
   (* an empty map for a block *)
   Definition empty_in_phi_info :=
-    in_phi_info [] [] (NoDup_nil YULVariable.t) (eq_refl (length [])).
+    in_phi_info [] [] (NoDup_nil VarID.t) (eq_refl (length [])).
 
   (* The empty phi function maps every block ID to the empty map. *)
   Definition empty :=  
       fun bid : BlockID.t => empty_in_phi_info.
 
-  Program Definition construct (out_vars: list YULVariable.t) (in_vars: list SimpleExprD.t) : option InBlockPhiInfo :=
-    match Misc.nodupb YULVariable.t YULVariable.eqb out_vars with
-    | false => None
+  (* IMPORTANT: when there is an error, it uses a defualt value
+  instead of failing. It is done this way so the current parser keeps
+  working, should be changed one the new parser is tready *)
+  Program Definition construct (out_vars: list VarID.t) (in_vars: list SimpleExprD.t) :  InBlockPhiInfo :=
+    match Misc.nodupb VarID.t VarID.eqb out_vars with
+    | false => empty_in_phi_info
     | true => match Nat.eqb (length out_vars) (length in_vars) with
-              | false => None
-              | true  => Some (in_phi_info out_vars in_vars _ _)
+              | false => empty_in_phi_info
+              | true  => (in_phi_info out_vars in_vars _ _)
               end
     end.
   Next Obligation.
     apply Is_true_eq_right in Heq_anonymous0.
-    apply (Misc.nodupb_spec YULVariable.t YULVariable.eqb YULVariable.eqb_eq YULVariable.eq_dec) in Heq_anonymous0.
+    apply (Misc.nodupb_spec VarID.t VarID.eqb VarID.eqb_eq VarID.eq_dec) in Heq_anonymous0.
     exact Heq_anonymous0.
   Defined.
 
@@ -299,11 +300,10 @@ Module PhiInfo (D: DIALECT).
     exact Heq_anonymous.
   Defined.
 
-
 End PhiInfo.
 
 
-Module Instruction (D: DIALECT).
+Module Instr (D: DIALECT).
   Module SimpleExprD := SimpleExpr(D).
 
   Inductive aux_inst_t :=
@@ -312,33 +312,30 @@ Module Instruction (D: DIALECT).
   (* An instruction is a pair of a block ID and a YUL variable. *)
   Record t : Type := {
       input : list SimpleExprD.t; 
-      output : list YULVariable.t; (* Output variables *)
-      op : (FunctionName.t + D.opcode_t) + aux_inst_t;
+      output : list VarID.t; (* Output variables *)
+      op : (FuncID.t + D.opcode_t) + aux_inst_t;
       H_nodup : NoDup output;
     }.
   
-  Program Definition construct (input : list SimpleExprD.t) (output : list YULVariable.t) (op : (FunctionName.t + D.opcode_t) + aux_inst_t) : option t :=
-  match Misc.nodupb YULVariable.t YULVariable.eqb output with
-  | true => Some ({| input:= input; output:=output; op:= _ |})
-  | false => None
+  (* IMPORTANT: when there is an error, it uses a defualt value
+  instead of failing. It is done this way so the current parser keeps
+  working, should be changed one the new parser is tready *)
+  Program Definition construct (input : list SimpleExprD.t) (output : list VarID.t) (op : (FuncID.t + D.opcode_t) + aux_inst_t) : t :=
+  match Misc.nodupb VarID.t VarID.eqb output with
+  | true => {| input:= input; output:=output; op:= _ |}
+  | false => {| input:= []; output:=[]; op:=op; H_nodup := (NoDup_nil VarID.t) |}
   end.
 Next Obligation.
   apply Is_true_eq_right in Heq_anonymous.
-  apply (Misc.nodupb_spec YULVariable.t YULVariable.eqb YULVariable.eqb_eq YULVariable.eq_dec) in Heq_anonymous.
+  apply (Misc.nodupb_spec VarID.t VarID.eqb VarID.eqb_eq VarID.eq_dec) in Heq_anonymous.
   exact Heq_anonymous.
 Defined.
 
-End Instruction.
+End Instr.
 
-(*
-How to access the entries of an Instruction i of type Instruction(D).t? 
-- i.(Instruction.input) to access the input
-- i.(Instruction.output) to access the output
-- i.(Instruction.op) to access the operation
-*)
 
 Module Block (D: DIALECT).
-  Module InstructionD := Instruction(D). (* Required to access Instruction(D) *)
+  Module InstrD := Instr(D). (* Required to access Instr(D) *)
   Module PhiInfoD := PhiInfo(D).
   Module ExitInfoD := ExitInfo(D).
   
@@ -347,10 +344,10 @@ Module Block (D: DIALECT).
       bid : BlockID.t;
       phi_function : PhiInfoD.t;
       exit_info : ExitInfoD.t;
-      instructions : list (InstructionD.t); (* List of instructions in the block *)
+      instructions : list (InstrD.t); (* List of instructions in the block *)
     }.
 
-  Definition construct (bid: BlockID.t) (phi_function : PhiInfoD.t) (exit_info : ExitInfoD.t) (instructions : list (InstructionD.t)) :=
+  Definition construct (bid: BlockID.t) (phi_function : PhiInfoD.t) (exit_info : ExitInfoD.t) (instructions : list (InstrD.t)) :=
     {|
       bid := bid;
       phi_function := phi_function;
@@ -378,7 +375,7 @@ Module Block (D: DIALECT).
 
   Definition is_terminated_block (b : t) :=
     match b.(exit_info) with
-    | ExitInfoD.Terminated => true
+    | ExitInfoD.Terminate => true
     | _ => false
     end.
 
@@ -386,30 +383,29 @@ End Block.
 
 
 
-Module Function (D: DIALECT).
+Module CFGFun (D: DIALECT).
   Module BlockD := Block(D). (* Required to access Block(D) *)
   
     (* A function is a collection of blocks, an entry block ID, and a name. *)
   Record t : Type := {
-      name : FunctionName.t;
-      arguments : list YULVariable.t; (* Input parameters *)
+      name : FuncID.t;
+      args : list VarID.t; (* Input parameters *)
       blocks : list BlockD.t; (* List of blocks *)
-      entry_block_id : BlockID.t; (* The ID of the entry block. *)
-      H_nodup : NoDup arguments
+      entry_bid : BlockID.t; (* The ID of the entry block. *)
+      H_nodup : NoDup args
     }.
 
-  Program Definition construct (name : FunctionName.t) (arguments : list YULVariable.t) (blocks : list BlockD.t) (entry_block_id : BlockID.t) :=
-    match Misc.nodupb YULVariable.t YULVariable.eqb arguments with
-    | false => None
-    | true => Some {| name := name; blocks := blocks; entry_block_id := entry_block_id; H_nodup := _ |}
+  Program Definition construct (name : FuncID.t) (args : list VarID.t) (blocks : list BlockD.t) (entry_bid : BlockID.t) : t :=
+    match Misc.nodupb VarID.t VarID.eqb args with
+    | false => {| name := name; blocks := []; entry_bid := entry_bid; H_nodup := (NoDup_nil VarID.t)|}
+    | true => {| name := name; blocks := blocks; entry_bid := entry_bid; H_nodup := _ |}
     end.
   Next Obligation.
     apply Is_true_eq_right in Heq_anonymous.
-    apply (Misc.nodupb_spec YULVariable.t YULVariable.eqb YULVariable.eqb_eq YULVariable.eq_dec) in Heq_anonymous.
+    apply (Misc.nodupb_spec VarID.t VarID.eqb VarID.eqb_eq VarID.eq_dec) in Heq_anonymous.
     exact Heq_anonymous.
   Defined.
 
-      
   Definition get_block (f: t) (bid: BlockID.t) : option BlockD.t :=
     match List.find (fun b => BlockID.eqb b.(BlockD.bid) bid) f.(blocks) with
     | Some block => Some block
@@ -419,56 +415,57 @@ Module Function (D: DIALECT).
   Definition valid_function (f: t) :=
     forall b,
       In b (blocks f) <-> get_block f b.(BlockD.bid) = Some b.
-   
-End Function.
+
+End CFGFun.
 
 
-Module SmartContract (D: DIALECT).
-  Module FunctionD := Function(D). (* Required to access Function(D) *)
-  Module BlockD := FunctionD.BlockD.
+Module CFGProg (D: DIALECT).
+  Module CFGFunD := CFGFun(D). (* Required to access Function(D) *)
+  Module BlockD := CFGFunD.BlockD.
+  Module InstrD := BlockD.InstrD.
   
   (* A smart contract is a collection of functions and a main function. *)
   Record t : Type := {
     name : string; (* Name of the smart contract *)
-    functions : list FunctionD.t; (* List of functions in the smart contract *)
-    main: FunctionName.t; (* The main function of the smart contract *)
+    functions : list CFGFunD.t; (* List of functions in the smart contract *)
+    main: FuncID.t; (* The main function of the smart contract *)
   }.
 
-  Definition construct (name : string) (functions : list FunctionD.t) (main: FunctionName.t) :=
+  Definition construct (name : string) (functions : list CFGFunD.t) (main: FuncID.t) : t :=
     {| name := name; functions := functions; main := main |}.
 
-  Definition get_function (sc: t) (fname: FunctionName.t) : option FunctionD.t :=
-    match List.find (fun f => FunctionName.eqb f.(FunctionD.name) fname) sc.(functions) with
+  Definition get_func (sc: t) (func_id: FuncID.t) : option CFGFunD.t :=
+    match List.find (fun f => FuncID.eqb f.(CFGFunD.name) func_id) sc.(functions) with
     | Some func => Some func
     | None => None
     end.
 
-  Definition get_block (sc: t) (fname: FunctionName.t) (bid: BlockID.t) : option BlockD.t :=
-    match get_function sc fname with
-    | Some func => FunctionD.get_block func bid
+  Definition get_block (sc: t) (func_id: FuncID.t) (bid: BlockID.t) : option BlockD.t :=
+    match get_func sc func_id with
+    | Some func => CFGFunD.get_block func bid
     | None => None
     end.
 
-  Definition get_instruction (sc: t) (fname: FunctionName.t) (bid: BlockID.t) (index: nat) : option BlockD.InstructionD.t :=
-    match get_block sc fname bid with
+  Definition get_instr (sc: t) (func_id: FuncID.t) (bid: BlockID.t) (index: nat) : option InstrD.t :=
+    match get_block sc func_id bid with
     | Some block =>
         List.nth_error block.(BlockD.instructions) index 
     | None => None
     end.
 
-  Definition get_first_block_id (sc: t) (fname: FunctionName.t) : option BlockID.t :=
-    match get_function sc fname with
-    | Some func => Some func.(FunctionD.entry_block_id)
+  Definition get_entry_bid (sc: t) (func_id: FuncID.t) : option BlockID.t :=
+    match get_func sc func_id with
+    | Some func => Some func.(CFGFunD.entry_bid)
     | None => None
     end.
 
   Definition all_function_name_are_different  (p: t) :=
       forall f,
-        In f (functions p) <-> get_function p f.(FunctionD.name) = Some f.
+        In f (functions p) <-> get_func p f.(CFGFunD.name) = Some f.
 
   Definition all_function_are_valid  (p: t) :=
     forall f,
-      In f (functions p) -> FunctionD.valid_function f.
+      In f (functions p) -> CFGFunD.valid_function f.
 
   Definition valid_smart_contract (p: t) :=
     all_function_name_are_different p /\ all_function_are_valid p.
@@ -476,30 +473,30 @@ Module SmartContract (D: DIALECT).
   Lemma valid_p_vs_get_block:
     forall p,
       valid_smart_contract p ->
-      forall fname bid b,
-        get_block p fname bid = Some b <->
-          exists f, In f p.(functions)  /\ In b f.(FunctionD.blocks) /\ FunctionName.eqb f.(FunctionD.name) fname = true /\ BlockID.eqb b.(BlockD.bid) bid = true.
+      forall func_id bid b,
+        get_block p func_id bid = Some b <->
+          exists f, In f p.(functions)  /\ In b f.(CFGFunD.blocks) /\ FuncID.eqb f.(CFGFunD.name) func_id = true /\ BlockID.eqb b.(BlockD.bid) bid = true.
   Proof.
     intros p H_valid_p.
     intros f bid b.
     split.
     - intros H_get_block.
       unfold get_block in H_get_block.
-      destruct (get_function p f) as [func|] eqn:E_get_function; try discriminate.
-      unfold get_function in E_get_function.
-      destruct (find (fun f0 : FunctionD.t => FunctionName.eqb (FunctionD.name f0) f)) as [func'|] eqn:E_find_func'; try discriminate.
-      injection E_get_function as H_func'_eq_func.
+      destruct (get_func p f) as [func|] eqn:E_get_func; try discriminate.
+      unfold get_func in E_get_func.
+      destruct (find (fun f0 : CFGFunD.t => FuncID.eqb (CFGFunD.name f0) f)) as [func'|] eqn:E_find_func'; try discriminate.
+      injection E_get_func as H_func'_eq_func.
       subst func'.
 
-      unfold FunctionD.get_block in H_get_block.
-      destruct (find (fun b : FunctionD.BlockD.t => BlockID.eqb (FunctionD.BlockD.bid b) bid) (FunctionD.blocks func)) as [b'|] eqn:E_find_b'; try discriminate.
+      unfold CFGFunD.get_block in H_get_block.
+      destruct (find (fun b : CFGFunD.BlockD.t => BlockID.eqb (CFGFunD.BlockD.bid b) bid) (CFGFunD.blocks func)) as [b'|] eqn:E_find_b'; try discriminate.
         
       injection H_get_block as H_b'_eq_b.
       subst b'.
 
-      pose proof (find_some (fun f0 : FunctionD.t => FunctionName.eqb (FunctionD.name f0) f) (functions p) E_find_func' ) as [H_in_func_pfs H_func_name_eqb_f].
+      pose proof (find_some (fun f0 : CFGFunD.t => FuncID.eqb (CFGFunD.name f0) f) (functions p) E_find_func' ) as [H_in_func_pfs H_func_name_eqb_f].
       
-      pose proof (find_some (fun b : FunctionD.BlockD.t => BlockID.eqb (FunctionD.BlockD.bid b) bid) (FunctionD.blocks func) E_find_b') as [H_in_b_funcbs H_b_bid_eqb_bid].
+      pose proof (find_some (fun b : CFGFunD.BlockD.t => BlockID.eqb (CFGFunD.BlockD.bid b) bid) (CFGFunD.blocks func) E_find_b') as [H_in_b_funcbs H_b_bid_eqb_bid].
 
       exists func.
       repeat split.
@@ -511,7 +508,7 @@ Module SmartContract (D: DIALECT).
     - intros H_exists_f0.
       destruct H_exists_f0 as [f0 [In_f0_pfs [In_b_f0bs [H_f0_name_eqb_f H_b_bid_eqb_b]]]].
 
-      apply FunctionName.eqb_eq in H_f0_name_eqb_f.
+      apply FuncID.eqb_eq in H_f0_name_eqb_f.
       subst f.
 
       apply BlockID.eqb_eq in H_b_bid_eqb_b.
@@ -519,23 +516,23 @@ Module SmartContract (D: DIALECT).
       
       
       unfold valid_smart_contract in H_valid_p.
-      destruct H_valid_p as [H_all_fname_diff H_all_f_valid].
+      destruct H_valid_p as [H_all_func_id_diff H_all_f_valid].
 
       
-      unfold all_function_name_are_different in H_all_fname_diff.
+      unfold all_function_name_are_different in H_all_func_id_diff.
       unfold all_function_are_valid in H_all_f_valid.
 
       unfold get_block.
 
-      pose proof (H_all_fname_diff f0) as H_get_function_f0.
+      pose proof (H_all_func_id_diff f0) as H_get_func_f0.
       pose proof (H_all_f_valid f0 In_f0_pfs) as H_f0_valid.
-      unfold FunctionD.valid_function in H_f0_valid.
+      unfold CFGFunD.valid_function in H_f0_valid.
 
-      rewrite H_get_function_f0 in In_f0_pfs.
+      rewrite H_get_func_f0 in In_f0_pfs.
       rewrite In_f0_pfs.
       
       rewrite H_f0_valid in In_b_f0bs.
       apply In_b_f0bs.
   Qed.
 
-End SmartContract.
+End CFGProg.
