state.v
@@ -1,106 +1,68 @@
 Require Export FORYU.list_functions.
 Require Export FORYU.program.
- 
-Module VariableAssignment(D: DIALECT).
 
-  Module YULVariableMapD := YULVariableMap(D).
+Module Locals(D: DIALECT).
+
   Module SimpleExprD := SimpleExpr(D).
 
-  (* Assignment from YUL variables to dialect values *)
-  Definition t := YULVariable.t -> D.value_t.
-  (* Variables not initialized return the default value of the dialect *)
+  (* Mapping from YUL local variables to dialect values -- we have
+  infinite number of registers*)
+  Definition t := VarID.t -> D.value_t.
 
+  (* VarIDiables not initialized return the default value of the dialect
+  *)
   Definition empty : t := fun _ => D.default_value.
 
-  Definition assign (assignments : t) (var : YULVariable.t) (value : D.value_t) : t :=
-    fun v => if YULVariable.eqb v var then value else assignments v.
+  (* sets the value of [var] to [value] in [locals] *)
+  Definition set (locals : t) (var : VarID.t) (value : D.value_t) : t :=
+    fun v => if VarID.eqb v var then value else locals v.
 
-  Definition get (assignments : t) (var : YULVariable.t) : D.value_t :=
-    assignments var.
-
-  (* This get recieves a list of simple expressions *)
-  Definition get_se (assignments : t) (e : SimpleExprD.t) : D.value_t :=
-    match e with
-    | inl var => assignments var
-    | inr val => val
-    end.
-
-  (* Returns a list of values for the given variables, if all variables are assigned. *)
-  (* If any variable is not assigned, returns None. *)
-  Definition get_all (assignments : t) (vars : list YULVariable.t) : list D.value_t :=
-    List.map (fun v => get assignments v) vars.
-
-  Definition get_all_se (assignments : t) (es : list SimpleExprD.t) : list D.value_t :=
-    List.map (fun e => get_se assignments e) es.
-
-  (* Takes a list of variables and a list of values and updates the assignment. If the list have 
-     different lengths, returns None  *)
-  Fixpoint assign_all (assignments : t) (vars : list YULVariable.t) (vals : list D.value_t) : option t :=
+  (* Takes a list of variables and a list of values and updates sets
+     all of them. If the lists have different lengths, returns None *)
+  Fixpoint set_all (locals : t) (vars : list VarID.t) (vals : list D.value_t) : option t :=
     match vars, vals with
-    | nil, nil => Some assignments
+    | nil, nil => Some locals
     | nil, _ :: _ => None
     | _ :: _, nil => None
     | var :: rvars, val :: rvals =>
-        let new_assignments := assign assignments var val in
-        assign_all new_assignments rvars rvals
-    (*
-        match assign_all assignments rvars rvals with
-        | Some new_assignments => Some (assign new_assignments var val)
-        | None => None
-        end
-     *) 
+        let locals' := set locals var val in
+        set_all locals' rvars rvals
     end.
 
-  (* Applies a list of renamings to the assignments. Each renaming is a pair (dest, origin) where 
-     dest is the variable that will take the value of origin. *)
-  Fixpoint apply_renamings (assignments : t) (renamings : YULVariableMapD.t) : t :=
-    match renamings with
-    | nil => assignments
-    | (dest, origin) :: rest =>
-        apply_renamings (assign assignments dest (get_se assignments origin)) rest
-    end.
+  (* returns the value of [var] in [locals] *)
+  Definition get (locals : t) (var : VarID.t) : D.value_t :=
+    locals var.
 
-End VariableAssignment.
+  (* Returns a list of values for the given variables *)
+  Definition get_all (locals : t) (vars : list VarID.t) : list D.value_t :=
+    List.map (fun v => get locals v) vars.
+
+
+End Locals.
 
 
 Module StackFrame(D: DIALECT).
   (* Stack frame for a function call *)
-  Module VariableAssignmentD := VariableAssignment(D).
-  (* Module SmartContractD := SmartContract(D). *)
-  
+  Module LocalsD := Locals(D).
   
   Record t : Type := {
-    function_name : FunctionName.t;
-    variable_assignments : VariableAssignmentD.t;
-    (* curr_block : BlockD.t; (* current block in execution, the list of instructions is consumed *) *)
-    (*curr_block : SmartContractD.BlockD.t; (* current block in execution, the list of instructions is consumed *)*)
-    curr_block_id: BlockID.t; (* id of the current block *)
-    pc : nat; (* position of the next instructions in the curr_block *)
-  }.
-
-  Definition increase_pc (sf: t) : t :=
-    {| 
-      function_name := sf.(function_name);
-      variable_assignments := sf.(variable_assignments);
-      curr_block_id := sf.(curr_block_id);
-      pc := sf.(pc) + 1;
-    |}.
+      func_id : FuncID.t;
+      locals : LocalsD.t;
+      curr_bid: BlockID.t; (* id of the current block *)
+      pc : nat; (* position of the next instructions in the current block. We keep using nat becuase there are many code/theorems we need that do not exists for N. Idieally we shoukd use N for efficiency in the different analysis. *)
+    }.
+ 
 End StackFrame.
+
 
 
 Module CallStack(D: DIALECT).
   (* Stack of variable assignments for the calling functions *)
   Module StackFrameD := StackFrame(D).
+
   Definition t := list StackFrameD.t.
 
   Definition empty : t := nil.
-  Definition push (call_stack : t) (assignments : StackFrameD.t) : t :=
-    assignments :: call_stack.
-  Definition pop (call_stack : t) : t :=
-    match call_stack with
-    | nil => nil
-    | _ :: rest => rest
-    end.
 End CallStack.
 
 
@@ -108,37 +70,34 @@ Module State(D: DIALECT).
   (* State of the program *)
   Module CallStackD := CallStack(D).
   Module StackFrameD := CallStackD.StackFrameD.
-  Module VariableAssignmentD := StackFrameD.VariableAssignmentD.
-(*  Module SmartContractD := SmartContract(D). *)
+  Module LocalsD := StackFrameD.LocalsD.
     
   Record t : Type := {
     call_stack : CallStackD.t;
     status : Status.t;
-    dialect_state : D.dialect_state;
+    dialect_state : D.dialect_state_t;
   }.
 
-  Definition empty : t := {|
-    call_stack := CallStackD.empty;
-    status := Status.Running;
-    dialect_state := D.empty_dialect_state;
-  |}.
-
-  (* State with with a stack frame to start block #0 of the "main" function, with pc=0 *)
-  Definition initial_main : t := {|
-    call_stack := ({| StackFrameD.function_name := "main"%string;
-                      StackFrameD.variable_assignments := VariableAssignmentD.empty;
-                      StackFrameD.curr_block_id := 0%nat;
-                      StackFrameD.pc := 0%nat;
-                   |} ) :: nil;
-    status := Status.Running;
-    dialect_state := D.empty_dialect_state;
-  |}.
-
-  Definition set_status (s: t) (new_status: Status.t) : t :=
+  Definition set_status (s: t) (status: Status.t) : t :=
     {| 
       call_stack := s.(call_stack);
-      status := new_status;
+      status := status;
       dialect_state := s.(dialect_state);
     |}.
 
+  Definition set_dialect_state (s: t) (dialect_state: D.dialect_state_t) : t :=
+    {| 
+      call_stack := s.(call_stack);
+      status := s.(status);
+      dialect_state := dialect_state;
+    |}.
+
+  Definition set_call_stack (s: t) (call_stack': CallStackD.t) : t :=
+    {| 
+      call_stack := call_stack';
+      status := s.(status);
+      dialect_state := s.(dialect_state)
+    |}.
+
 End State.
+
